$\ce{A<=>[k_1][k_2]R}$
$M =\frac{C_{R0}}{C_{A0}}$
$C_A = C_{A0}(1-x_A)$
$C_R = C_{R0}+C_{A0}x_A = C_{A0}(M+x_A)$
$\frac{dC_A}{dt} = -k_1C_A+k_2C_R$
$-C_{A0}\frac{dx_A}{dt} = -k_1C_{A0}(1-x_A)+k_2C_{A0}(M+x_A)$
at equilibrium, rate = 0,
$x_{A\ eq} = \frac{k_1-Mk_2}{k_1+k_2}$

$\ce{A+B<=>[k_1][k_2]R+S}$





















































































































































































































































































































































































